\section{Elliptic Curve Arithmetic}
\label{section:ec}

\subsection{Unified Incomplete Addition and Doubling}

\begin{center}
    \begin{table}[H]
        \begin{tabular}{llllllllllllllll}
            Row   & 0     & 1     & 2     & 3     & 4     & 5     & 6   & 7       & 8       & 9       & 10      & 11      & 12      & 13      & 14      \\
            $i$ & $x_1$ & $y_1$ & $x_2$ & $y_2$ & $x_3$ & $y_3$ & $\texttt{inf}$ & $\texttt{same\_x}$ & $s$ & $\texttt{inv}_y$ & $\texttt{inv}_x$ & $\dots$ & $\dots$ & $\dots$ & $\dots$ \\
        \end{tabular}
    \end{table}
\end{center}

Evaluations:
\begin{itemize}
	\item Addition case:
	\begin{itemize}
		\item $(x_3, y_3) = (x_1, y_1) + (x_2, y_2)$
		\item $\texttt{inf} = 1$ if $(x_3, y_3)$ is a point-at-infinity, $\texttt{inf} = 0$ otherwise
		\item $\texttt{same\_x} = 1$ if $x_1 = x_2$, $\texttt{same\_x} = 0$ otherwise
		\item $s = \frac{y_1 - y_2}{x_1 - x_2}$ if $x_1 \neq x_2$, $s = 0$ otherwise
		\item $\texttt{inv}_y = \frac{1}{y_2 - y_1}$ if $y_2 \neq y_1$, $\texttt{inv}_y = 0$ otherwise 
		\item $\texttt{inv}_x = \frac{1}{x_2 - x_1}$ if $x_2 \neq x_1$, $\texttt{inv}_x= 0$ otherwise
	\end{itemize}
	\item Doubling case:
	\begin{itemize}
		\item $(x_3, y_3) = 2(x_1, y_1)$
		\item $x_2 = x_1$, $y_2 = y_1$
		\item $\texttt{inf} = 1$ if $(x_3, y_3)$ is a point-at-infinity, $\texttt{inf} = 0$ otherwise
		\item $\texttt{same\_x} = 1$
		\item $s = \frac{3x_1^2}{2y_1}$ if $y_1 \neq 0$, $s = 0$ otherwise
		\item $\texttt{inv}_y = 0$ 
		\item $\texttt{inv}_x= 0$
	\end{itemize}
\end{itemize}

Constraints ($\textbf{max degree} = 3$):
\begin{enumerate}
	 \item $w_7 \cdot (w_2 - w_0) = 0$
    \item $(w_2 - w_0) \cdot w_{10} - (1 - w_7) = 0$
    \item $w_7 \cdot (2w_8 \cdot w_1 - 3w_0^2) + (1 - w_7) \cdot ((w_2 - w_0) \cdot w_8 - (w_3 - w_1))$
    \item $w_8^2 = w_0 + w_2 + w_4$
    \item $w_5 = w_8 \cdot (w_0 - w_4) - w_1$
    \item $(w_3 - w_1) \cdot (w_7 - w_6) = 0$
    \item $(w_3 - w_1) \cdot w_9 - w_6 = 0$
\end{enumerate}

Copy constraints:
\begin{enumerate}
	\item $w_6 = 0$
\end{enumerate}

\paragraph{Details.}

The gate uses basic group law formulae. 
Let $P = (x_1, y_1), Q = (x_2, y_2), R = (x_3, y_3)$ and $R = P + Q$. Then: 
\begin{itemize}
    \item $(x_2 - x_1) \cdot s = y_2 - y_1$
    \item $s^2 = x_1 + x_2 + x_3$
    \item $y_3 = s \cdot (x_1 - x_3) - y_1$
\end{itemize}
For point doubling $R = P + P = 2P$:
\begin{itemize}
    \item $2s \cdot y_1 = 3x_1^2$
    \item $s^2 = 2x_1 + x_3$
    \item $y_3 = s \cdot (x_1 - x_3) - y_1$
\end{itemize}

The gate does not handle cases $\mathcal{O} + P$ or $\mathcal{O} + \mathcal{O}$.
To ensure that operations with point-at-infinity are not included in the circuit's trace, copy constraint $w_6 = 0$ ($\texttt{inf} = 0$) was introduced. 

Constraints details:
\begin{itemize}
	 \item $x_2 - x_1$ zero check:
	 \begin{enumerate}
		 	\item $w_7 \cdot (w_2 - w_0) = 0 \longleftrightarrow 
		 			\texttt{same\_x} \cdot (x_2 -x_1)$ \\
		 		If $x_1 \neq x_2$, then $\texttt{same\_x} = 0$
		    \item $(w_2 - w_0) \cdot w_{10} - (1 - w_7) = 0 \longleftrightarrow 
		    		(x_2 - x_1) \cdot \texttt{inv}_x - (1 - \texttt{same\_x})$ \\
		    	If $x_1 \neq x_2$, then $\texttt{inv}_x = (x_2 - x_1)^{-1}$
	 \end{enumerate}
	 \item Group law constraints:
	 \begin{enumerate}
	 	\item $w_7 \cdot (2w_8 \cdot w_1 - 3w_0^2) + (1 - w_7) \cdot ((w_2 - w_0 \cdot w_8 - (w_3 - w_1)) \longleftrightarrow$ \\
			  $\texttt{same\_x} \cdot (2s \cdot y_1 - 3x_1^2) + (1 - \texttt{same\_x}) \cdot (x_2 - x_1 \cdot s - (y_2 - y_1))$ \\
			If $x_1 = x_2$ then use doubling $2s \cdot y_1 = 3x_1^2$. Otherwise use addition $(x_2 - x_1) \cdot s = y_2 - y_1$.
	 	\item $w_8^2 = w_0 + w_2 + w_4 \longleftrightarrow 
	 			s^2 = x_1 + x_2 + x_3$ \\
	 		Constrains $x_3$. It does not depend on $x_1, x_2$ equality.
	 	\item $w_5 = w_8 \cdot (w_0 - w_4) - w_1 \longleftrightarrow 
	 			y_3 = s \cdot (x_1 - x_3) - y_1$ \\
	 		Constrains $y_3$. It does not depend on $x_1, x_2$ equality.
	 \end{enumerate}
	 \item $P + (-P)$ constraints:
	 \begin{enumerate}
		 \item $(w_3 - w_1) \cdot (w_7 - w_6) = 0 \longleftrightarrow 
	    			(y_2 - y_1) \cdot (\texttt{same\_x} - \texttt{inf}) = 0$ \\ 
	    	We can get inifinity point iff $x_1 = x_2$ and $y_1 \neq y_2$. \\
	    	If $y_1 \neq y_2$ then $\texttt{inf} = \texttt{same\_x}$.
	    \item $(w_3 - w_1) \cdot w_9 - w_6 = 0 \longleftrightarrow 
	    			(y_2 - y_1) \cdot \texttt{inv}_y - \texttt{inf}$ \\
	    	The prover sets $\texttt{inv}_y = 0$ for $y_1 = y_2$. \\
	    	If $y_1 \neq y_2$ then $\texttt{inv}_y = (y_2 - y_1)^{-1}$
	 \end{enumerate}
\end{itemize}

\subsection{Variable Base Scalar Multiplication}
For $R  = [r]T$, $k = \frac{x - 2^{255}}{2}$:
\footnote{Using the results from \url{https://arxiv.org/pdf/math/0208038.pdf}}
\begin{enumerate}
    \item $P = [2]T$
    \item for $i$ from $n - 1$ to $0$:
    \begin{enumerate}
        \item $Q = k_{i + 1} \: ? \: T : -T$
        \item $R = P + Q + P$
    \end{enumerate}
\end{enumerate}

The first and last steps of the alforithm are verified by the unified addition and doubling circuit. 

\begin{center}
    \begin{table}[H]
        \begin{tabular}{llllllllllllllll}
            Row     & 0        & 1        & 2        & 3        & 4        & 5        & 6        & 7        & 8        & 9        & 10       & 11       & 12       & 13       & 14       \\
            $i$    & $x_T$    & $y_T$    & $x_0$    & $y_0$    & $n = 0$    & $n'$    & $--$    & $x_1$    & $y_1$    & $x_2$    & $y_2$    & $x_3$    & $y_3$ & $x_4$ & $y_4$ \\
            $i + 1$   & $x_5$    & $y_5$    & $b_0$    & $b_1$    & $b_2$    & $b_3$    & $b_4$      & $s_0$    & $s_1$    & $s_2$    & $s_3$    & $s_4$    & $--$ & $--$ & $--$ \\
            $\vdots$  & $\vdots$ & $\vdots$ & $\vdots$ & $\vdots$ & $\vdots$ & $\vdots$ & $\vdots$ & $\vdots$ & $\vdots$ & $\vdots$ & $\vdots$ & $\vdots$ & $\vdots$ & $\vdots$ & $\vdots$ \\
            $i + 100$ & $x_T$    & $y_T$    & $x_0$    & $y_0$    & $n$    & $n'$    & $--$    & $x_1$    & $y_1$    & $x_2$    & $y_2$    & $x_3$    & $y_3$ & $x_4$ & $y_4$ \\
            $i + 101$ & $x_5$    & $y_5$    & $b_0$    & $b_1$    & $b_2$    & $b_3$    & $b_4$      & $s_0$    & $s_1$    & $s_2$    & $s_3$    & $s_4$    & $--$ & $--$ & $--$ \\
        \end{tabular}
    \end{table}
\end{center}

Evaluations:
\begin{itemize}
	\item $b_i$ are bits of the $k$, first $b_1$ is the most significant bit of $k$, $n$ is an accumulator of $b_i$.
	\item $(x_1, y_1) - (x_0, y_0) = (x_0, y_0) + (x_T, (2b_1 - 1)y_T)$
	\item $(x_2, y_2) - (x_1, y_1) = (x_1, y_1) + (x_T, (2b_1 - 1)y_T)$
	\item $(x_3, y_3) - (x_2, y_2) = (x_2, y_2) + (x_T, (2b_1 - 1)y_T)$
	\item $(x_4, y_4) - (x_3, y_3) = (x_3, y_3) + (x_T, (2b_1 - 1)y_T)$
	\item $(x_5, y_5) - (x_4, y_4) = (x_4, y_4) + (x_T, (2b_1 - 1)y_T)$
	\item $s_0 = \frac{y_0 - (2b_0 - 1) \cdot y_T}{x_0 - x_T}$
	\item $s_1 = \frac{y_1 - (2b_1 - 1) \cdot y_T}{x_1 - x_T}$
	\item $s_2 = \frac{y_2 - (2b_2 - 1) \cdot y_T}{x_2 - x_T}$
	\item $s_3 = \frac{y_3 - (2b_3 - 1) \cdot y_T}{x_3 - x_T}$
	\item $s_4 = \frac{y_4 - (2b_4 - 1) \cdot y_T}{x_4 - x_T}$
\end{itemize}

Constraints:
\begin{itemize}
    \item $\texttt{next}(w_2) \cdot (w_2 - 1) = 0$
    \item $\texttt{next}(w_3) \cdot (w_3 - 1) = 0$
    \item $\texttt{next}(w_4) \cdot (w_4 - 1) = 0$
    \item $\texttt{next}(w_5) \cdot (w_5 - 1) = 0$
    \item $\texttt{next}(w_6) \cdot (w_6 - 1) = 0$ \\

    \item $(w_{2} - w_{0}) \cdot \texttt{next}(w_7) = w_3 - (2\texttt{next}(w_{2}) - 1) \cdot w_1$
    \item $(w_{7} - w_{0}) \cdot \texttt{next}(w_8) = w_8 - (2\texttt{next}(w_{3}) - 1) \cdot w_1$
    \item $(w_{10} - w_{0}) \cdot \texttt{next}(w_9) = w_{11} - (2\texttt{next}(w_{4}) - 1) \cdot w_1$
    \item $(w_{12} - w_{0}) \cdot \texttt{next}(w_{10}) = w_{13} - (2\texttt{next}(w_{5}) - 1) \cdot w_1$
    \item $(\texttt{next}(w_{0}) - w_{0}) \cdot \texttt{next}(w_{11}) = \texttt{next}(w_1) - (2\texttt{next}(w_{6}) - 1) \cdot w_1$ \\
    
    
    \item $(2\cdot w_{3} - \texttt{next}(w_7) \cdot (2 \cdot w_2 - \texttt{next}(w_7)^2 + w_{0}))^2 =  (2 \cdot w_2 - \texttt{next}(w_7)^2 + w_{0})^2 \cdot (w_7 - w_0 + \texttt{next}(w_7)^2)$
    \item $(2\cdot w_{8} - \texttt{next}(w_8) \cdot (2 \cdot w_7 - \texttt{next}(w_8)^2 + w_{0}))^2 =  (2 \cdot w_7 - \texttt{next}(w_8)^2 + w_{0})^2 \cdot (w_9 - w_0 + \texttt{next}(w_8)^2)$
    \item $(2\cdot w_{10} - \texttt{next}(w_9) \cdot (2 \cdot w_9 - \texttt{next}(w_9)^2 + w_{0}))^2 =  (2 \cdot w_9 - \texttt{next}(w_9)^2 + w_{0})^2 \cdot (w_{11} - w_0 + \texttt{next}(w_9)^2)$
    \item $(2\cdot w_{12} - \texttt{next}(w_{10}) \cdot (2 \cdot w_{11} - \texttt{next}(w_{10})^2 + w_{0}))^2 =  (2 \cdot w_{11} - \texttt{next}(w_{10})^2 + w_{0})^2 \cdot (w_{13} - w_0 + \texttt{next}(w_{10})^2)$
    \item $(2\cdot w_{14} - \texttt{next}(w_{11}) \cdot (2 \cdot w_{13} - \texttt{next}(w_{11})^2 + w_{0}))^2 =  (2 \cdot w_{13} - \texttt{next}(w_{11})^2 + w_{0})^2 \cdot (\texttt{next}(w_0) - w_0 + \texttt{next}(w_{11})^2)$ \\
    
    \item $(w_{8} + w_{3}) \cdot (2 \cdot w_2 - \texttt{next}(w_7)^2 + w_{0}) = (w_2 - w_7) \cdot (2\cdot w_{3} - \texttt{next}(w_7) \cdot (2 \cdot w_2 - \texttt{next}(w_7)^2 + w_{0}))$
    \item $(w_{10} + w_{8}) \cdot (2 \cdot w_7 - \texttt{next}(w_8)^2 + w_{0}) = (w_7 - w_9) \cdot (2\cdot w_{8} - \texttt{next}(w_8) \cdot (2 \cdot w_7 - \texttt{next}(w_8)^2 + w_{0}))$
    \item $(w_{12} + w_{10}) \cdot (2 \cdot w_9 - \texttt{next}(w_9)^2 + w_{0}) = (w_9 - w_{11}) \cdot (2\cdot w_{10} - \texttt{next}(w_9) \cdot (2 \cdot w_9 - \texttt{next}(w_9)^2 + w_{0}))$
    \item $(w_{14} + w_{10}) \cdot  (2 \cdot w_{11} - \texttt{next}(w_{10})^2 + w_{0}) = (w_{11} - w_{13}) \cdot (2\cdot w_{12} - \texttt{next}(w_{10}) \cdot (2 \cdot w_{11} - \texttt{next}(w_{10})^2 + w_{0}))$
    \item $(\texttt{next}(w_{1}) + w_{14}) \cdot (2 \cdot w_{13} - \texttt{next}(w_{11})^2 + w_{0}) = (w_{13} - \texttt{next}(w_{0}) \cdot (2\cdot w_{14} - \texttt{next}(w_{11}) \cdot (2 \cdot w_{13} - \texttt{next}(w_{11})^2 + w_{0}))$ \\
    
    
    \item $w_5 = 32 \cdot (w_4) + 16 \cdot \texttt{next}(w_{2}) + 8 \cdot \texttt{next}(w_{3}) + 4 \cdot \texttt{next}(w_{4}) + 2 \cdot \texttt{next}(w_{5}) + \texttt{next}(w_{6})$
    \end{itemize}
    
    Copy constraints:
    \begin{itemize}
    \item $(x_T,y_T)$ in row $j$ are copy constrained with $(x_T,y_T)$ in row $j + 2$ 
    \item $(x_0,y_0)$ in row $i$ are copy constrained with values from the first doubling circuit
    \item $(x_0,y_0)$ in row $j, j \neq i$ are copy constrained with $(x_5,y_5)$ in row $j - 1$ 
    \item $n = 0$ in row $i$ and $n$ in the row $j, j \neq i$ is copy contrained with $n'$ in the row $j-2$
    \end{itemize}

\subsection{Variable Base Endo-Scalar Multiplication}

For $R  = [b]T$, where $b = [b_n ... b_0]$ and $b_i \in \{0, 1\}$:
 \footnote{Using the results from \url{https://eprint.iacr.org/2019/1021.pdf}}
\begin{enumerate}
    \item $P = [2](\phi(T) + T)$
    \item for $i$ from $\frac{\lambda}{2} - 1$ to $0$:
    \begin{enumerate}
        \item $Q = r_{2i + 1} \: ? \: \phi([2r_{2i} - 1]T) : [2r_{2i} - 1]T$
        \item $R - P = P + Q$
    \end{enumerate}
\end{enumerate}
The first step of the alforithm are verified by the doubling and unified addition circuit. 

\begin{center}
    \begin{table}[H]
        \begin{tabular}{llllllllllllllll}
            Row    & 0        & 1        & 2        & 3        & 4        & 5        & 6        & 7        & 8        & 9        & 10       & 11       & 12       & 13       & 14       \\
            $i$   & $x_T$    & $y_T$    & $--$    & $--$    & $x_P$    & $y_P$    & $n = 0$      & $x_R$    & $y_R$    & $s_1$    & $s_3$    & $b_1$    & $b_2$ & $b_3$ & $b_4$ \\
            $\vdots$ & $\vdots$ & $\vdots$ & $\vdots$ & $\vdots$ & $\vdots$ & $\vdots$ & $\vdots$ & $\vdots$ & $\vdots$ & $\vdots$ & $\vdots$ & $\vdots$ & $\vdots$ & $\vdots$ & $\vdots$ \\
            $i + 63$ &  $x_T$    & $y_T$    & $--$    & $--$    & $x_P$    & $y_P$    & $n$      & $x_R$    & $y_R$    & $s_1$    & $s_3$    & $b_1$    & $b_2$ & $b_3$ & $b_4$ \\
            $i + 64$ &  $--$    & $--$    & $--$    & $--$    & $x_P$    & $y_P$    & $n$      & $--$    & $--$    & $--$    & $--$    & $--$    & $--$ & $--$ & $--$ \\
        \end{tabular}
    \end{table}
\end{center}

Evaluations:
\begin{itemize}
	\item The first $x_P, y_P$ are equal to $2 \cdot ((x_T, y_T) + ((\texttt{endo}) \cdot x_T, y_T))$
	\item $b_i$ are bits of the $k$, first $b_1$ is the most significant bit of $k$, $n$ is an accumulator of $b_i$.
	\item $(x_R, y_R) - (x_P, y_P) = (x_P, y_P) + (1 + (\texttt{endo} - 1) \cdot b_2) x_T, (2b_1 - 1)y_T)$
	\item $(\texttt{next}(x_P), \texttt{next}(y_P)) - (x_R, y_R) = (x_R, y_R) + ((\texttt{endo} - 1) \cdot b_2) x_T, (2b_1 - 1)y_T)$
	\item $s_1 = \frac{(2b_1 - 1) \cdot y_T - y_P}{(1 + (\texttt{endo} - 1) \cdot b_2) x_T - x_P}$
	\item $s_3 = \frac{(2b_1 - 1) \cdot y_T - y_R}{(1 + (\texttt{endo} - 1) \cdot b_2) x_T - x_R}$

\end{itemize}

Constraints:
\begin{itemize}
    \item $w_{11} \cdot (w_{11} - 1) = 0$
    \item $w_{12} \cdot (w_{12} - 1) = 0$
    \item $w_{13} \cdot (w_{13} - 1) = 0$
    \item $w_{14} \cdot (w_{14} - 1) = 0$
    \item $((1 + (\texttt{endo} - 1) \cdot w_{12}) \cdot w_{0} - w_{4}) \cdot w_{9} = (2 \cdot w_{11} - 1) \cdot w_{1} - w_{5}$
    \item $(2 \cdot w_{4} - w_{9}^2 + (1 + (\texttt{endo} - 1) \cdot w_{12}) \cdot w_{0}) \cdot ((w_{4} - w_{7}) \cdot w_{9} + w_{8} + w_{5}) = (w_{4} - w_{7}) \cdot 2 \cdot w_{5}$
    \item $(w_{8} + w_{5})^2 = (w_{4} - w_{7})^2 \cdot (w_{9}^2 - (1 + (\texttt{endo} - 1) \cdot w_{12}) \cdot w_{0} + w_{7})$
    \item $((1 + (\texttt{endo} - 1) \cdot w_{12}) \cdot w_{0} - w_{7}) \cdot w_{10} = (2 \cdot w_{13}-1) \cdot w_{1} - w_{8}$
    \item $(2 \cdot w_{7} - w_{10}^2 + (1 + (\texttt{endo} - 1) \cdot w_{14}) \cdot w_{0}) \cdot ((w_{7} - \texttt{next}(w_{4})) \cdot w_{10} + \texttt{next}(w_{5}) + w_{8}) = (w_{7} - \texttt{next}(w_{4})) \cdot 2 \cdot w_{8}$
    \item $(\texttt{next}(w_{4}) + w_{8})^2 = (w_{7} - \texttt{next}(w_{4}))^2 \cdot (w_{10}^2 - (1 + (\texttt{endo} - 1) \cdot w_{14}) \cdot w_{0} + \texttt{next}(w_{4}))$
    \item $\texttt{next}(w_{6}) = 16 \cdot w_{6} + 8 \cdot w_{11} + 4 \cdot w_{12} + 2 \cdot w_{13} + w_{14}$
\end{itemize}

    Copy constraints:
    \begin{itemize}
    \item $(x_T,y_T)$ in row $j$ are copy constrained with $(x_T,y_T)$ in row $j + 1$ 
    \item $(x_P,y_P)$ in row $i$ are copy constrained with values from the first doubling circuit
    \end{itemize}